Add reconstruction proof for `VarInt`s
TODO: the current proof is ugly and undocumented, fix

TODO: New parser broke roundtrip proof for `VarInt`, fix

LeanMqtt/Packets/VarHeader/Property/Basic.lean
@@ -1,3 +1,4 @@
+import LeanMqtt.Core.WithByteSize
 import LeanMqtt.Primitives.Basic
 
 namespace Mqtt
@@ -87,50 +88,5 @@ def Property.parser : Parser Property := do
 def Property.byteSize (p : Property) : Nat :=
   p.serialize.length
 
-/- ========================= Properties ========================= -/
-
-instance : GetLength (List Property) where
-  length l := l.foldl (fun acc p => acc + (Property.serialize p).length) 0 -- Placeholder, will be fixed
-
-abbrev Properties := WithLength (List Property) VarInt
-
-def Properties.serialize (ps : Properties) : List UInt8 :=
-  VarInt.serialize ps.len ++
-  ps.val.foldl (fun acc p => acc ++ p.serialize) []
-
-def parsePropsLoop (input : List UInt8) : Option (List Property) :=
-  if /-h_empty :-/ input.isEmpty then
-    some []
-  else
-    -- Run the parser manually on the current list
-    match Property.parser.run input with
-    | some (p, rest) =>
-      -- CRITICAL: We explicitly check that the parser consumed at least 1 byte.
-      -- This guarantees 'rest' is strictly smaller than 'input'.
-      -- TODO: we may be able to derive this check instead performing it
-      if /-h_progress :-/ rest.length < input.length then
-        match parsePropsLoop rest with
-        | some tail => some (p :: tail)
-        | none      => none
-      else
-        -- Parser succeeded but consumed 0 bytes (infinite loop risk).
-        -- Treat as an error.
-        none
-    | none => none
-termination_by input.length
-
-def Properties.parser : Parser Properties := do
-  -- 1. Parse the Length Prefix
-  let len ← VarInt.parser
-  let ⟨chunk, h_chunk_len⟩ ← bytesParserWithProof len
-
-  match h_parsed : parsePropsLoop chunk with
-  | some props =>
-    have h_len : len.val = (props.foldl (fun acc p => acc + p.byteSize) 0) := by
-      -- This proof will need to be fixed.
-      sorry
-
-    return { val := props, len := ⟨len, sorry⟩ }
-  | none => none
-
-end Mqtt
+instance : GetByteSize Property where
+  byteSize := Property.byteSize
