LeanMqtt/Core/WithByteSize.lean
@@ -1,0 +1,36 @@
+class GetByteSize (α : Type u) where
+  byteSize : α → Nat
+
+/-- In MQTT, a String's length is actually the number of bytes it contains. -/
+@[reducible]
+instance instStringByteLength : GetByteSize String where
+  byteSize s := s.utf8ByteSize
+
+-- @[reducible]
+-- instance : GetByteSize String where
+--   length := String.length
+
+@[reducible]
+instance : GetByteSize (Array UInt8) where
+  byteSize := Array.size
+
+-- @[reducible]
+-- instance {α} : GetByteSize (Array α) where
+--   length := Array.size
+
+-- class LengthEmbedding (lenTyp : Type) where
+--   toNat : lenTyp → Nat
+--   injective : Function.Injective toNat
+
+structure WithByteSize (α lenTyp) [s : GetByteSize α] [Coe lenTyp Nat] where
+  val : α
+  -- TODO: `Coe lenTyp Nat`, possible point of failure?
+  -- Example: for lenTyp = Int, `-5`.toNat.toInt ≠ `-5`
+  -- Fix: use LengthEmbedding instead of `Coe lenTyp Nat`
+  len : { n : lenTyp // n = s.byteSize val }
+
+@[simp]
+theorem WithByteSize.len_eq {α lenTyp} [GetByteSize α] [Coe lenTyp Nat]
+  (w : WithByteSize α lenTyp) :
+  ↑w.len.val = GetByteSize.byteSize w.val :=
+  w.len.property
