LeanMqtt/Packets/VarHeader/Properties/Basic.lean
@@ -1,0 +1,70 @@
+import LeanMqtt.Primitives.Basic
+import LeanMqtt.Packets.VarHeader.Property.Basic
+import LeanMqtt.Packets.VarHeader.Property.Proofs
+
+namespace Mqtt
+open Mqtt
+
+/- ========================= Properties ========================= -/
+
+abbrev Properties.rawByteSize (l : List Property) : Nat
+  := (l.map Property.byteSize).sum
+
+instance : GetByteSize (List Property) where
+  byteSize := Properties.rawByteSize
+
+abbrev Properties := WithByteSize (List Property) VarInt
+
+def Properties.serialize (ps : Properties) : List UInt8 :=
+  -- VarInt.serialize ps.len ++
+  -- ps.val.foldl (fun acc p => acc ++ p.serialize) []
+  VarInt.serialize ps.len ++ ps.val.flatMap Property.serialize
+
+def parsePropsLoop (input : List UInt8) :
+  Option { ps : (List Property) // input.length = Properties.rawByteSize ps } :=
+  if h_empty : input.isEmpty then
+    some ⟨[], by
+      have h_len_zero : input.length = 0 := by grind
+      simp [h_len_zero, Properties.rawByteSize]
+    ⟩
+  else
+    match h_parse : Property.parser.run input with
+    | some (p, rest) =>
+      -- `h_progress` makes sure the function terminates
+      -- TODO: we might be able to remove the check
+      -- if rest.length < input.length then
+        match parsePropsLoop rest with
+        | some ⟨tail, h_tail_len⟩ =>
+          let h_len_ps : input.length = Properties.rawByteSize (p :: tail) := by
+            have h_consumed : input.length = p.byteSize + rest.length
+              := Property.parser_len_consumed input p rest h_parse
+            rw [h_tail_len] at h_consumed
+            exact h_consumed
+
+          some ⟨(p :: tail), h_len_ps⟩
+        | none => none
+      -- else
+        -- none
+    | none => none
+termination_by input.length
+decreasing_by
+  -- We can prove termination using `Property.byteSize_pos p`.
+  -- Since it is still using `sorry`, we keep the older code commented for now.
+  have h_consumed := Property.parser_len_consumed input p rest h_parse
+  have h_pos := Property.byteSize_pos p
+  omega
+
+def Properties.parser : Parser Properties := do
+  let len ← VarInt.parser
+  let ⟨chunk, h_chunk_len⟩ ← bytesParserWithProof len
+
+  match parsePropsLoop chunk with
+  | some ⟨props, h_loop_len⟩ =>
+    have h_len : len.val = (props.map Property.byteSize).sum := by
+      rw [← h_chunk_len]
+      exact h_loop_len
+
+    return { val := props, len := ⟨len, h_len⟩ }
+  | none => none
+
+end Mqtt
