LeanMqtt/Packets/VarHeader/Properties/Proofs.lean
@@ -1,0 +1,49 @@
+import LeanMqtt.Packets.VarHeader.Basic
+import LeanMqtt.Packets.VarHeader.Property.Basic
+import LeanMqtt.Packets.VarHeader.Property.Proofs
+import LeanMqtt.Packets.VarHeader.Properties.Basic
+import LeanMqtt.Packets.VarHeader.Variations
+import LeanMqtt.Primitives.Proofs
+
+open Mqtt
+
+-- TODO: prove
+-- theoremt parsePropsLoop_len (chunk : List UInt8) (l : List Property) :
+--   parsePropsLoop chunk = some l → chunk.length = (l.foldl (fun acc p => acc + p.byteSize) 0) := by
+--   -- simp [GetByteSize.byteSize]
+--   sorry
+
+theorem Properties.roundtrip (ps : Properties) (rest : List UInt8) :
+  Properties.parser.run (ps.serialize ++ rest) = some (ps, rest) := by
+  sorry
+
+def Var_Connect.roundtrip (v : Var_Connect) (rest : List UInt8) :
+  Var_Connect.parser.run (v.serialize ++ rest) = some (v, rest) := by
+  simp [Var_Connect.parser, Var_Connect.serialize]
+  simp [Str.roundtrip]
+  simp [UInt8.roundtrip]
+  simp [Properties.roundtrip]
+
+theorem Var_Connack.roundtrip (v : Var_Connack) (rest : List UInt8) :
+  Var_Connack.parser.run (v.serialize ++ rest) = some (v, rest) := by
+  simp [Var_Connack.parser, Var_Connack.serialize]
+  simp [UInt8.roundtrip, Properties.roundtrip]
+
+theorem Var_Publish.roundtrip {qos} (v : Var_Publish qos) (rest : List UInt8) :
+  (Var_Publish.parser qos).run (v.serialize ++ rest) = some (v, rest) := by
+  simp [Var_Publish.parser, Var_Publish.serialize]
+  simp [Str.roundtrip]
+
+  split
+  · next h_qos =>
+    -- Case: QoS > 0
+    simp [UInt16.roundtrip]
+    simp [Properties.roundtrip]
+  · next h_qos =>
+    -- Case: QoS == 0
+    simp [Properties.roundtrip]
+    congr
+    have h_zero : qos = 0 := by bv_decide
+    subst h_zero
+    simp
+    apply Subsingleton.elim () v.packet_id
