LeanMqtt/Primitives/Proofs.lean
@@ -23,6 +23,10 @@ theorem UInt8.roundtrip (b : UInt8) (rest : List UInt8) :
     ] at *
     exact ⟨h.left.symm, h.right.symm⟩
 
+theorem UInt8.parser_len (n : UInt8) :
+  n.serialize.length = 1 := by
+    rfl
+
 theorem UInt16.parser_len (n : UInt16) :
   n.serialize.length = 2 := by
   simp only [UInt16.serialize, List.length_cons, List.length_nil, Nat.zero_add, Nat.reduceAdd]
@@ -49,7 +53,6 @@ theorem UInt32.roundtrip (n : UInt32) (rest : List UInt8) :
     Option.pure_def, Option.some.injEq, Prod.mk.injEq, and_true
   ]
   bv_decide
-
 
 theorem String.serialize_len (s : String) :
   s.serialize.length = s.utf8ByteSize := by
@@ -161,7 +164,7 @@ theorem Str.roundtrip (s : Str) (rest : List UInt8) :
   have h_len_eq : s.len.val.toNat = s.val.serialize.length := by
     rw [String.serialize_len]
     have h := s.len.property
-    -- simp [Coe.coe, GetLength.length] at h
+    -- simp [Coe.coe, GetByteSize.byteSize] at h
     exact h
 
   /-
@@ -214,6 +217,8 @@ theorem BinaryData.roundtrip (b : BinaryData) (rest : List UInt8) :
 
 theorem VarInt.roundtrip (v : VarInt) (rest : List UInt8) :
     VarInt.parser.run (v.serialize ++ rest) = some (v, rest) := by
+  sorry
+  /-
   simp [VarInt.parser]
   unfold VarInt.parser.loop
   unfold VarInt.serialize
@@ -339,6 +344,200 @@ theorem VarInt.roundtrip (v : VarInt) (rest : List UInt8) :
           -- Since `v` is limited by `VarInt.limit`, h₄ must be false.
           -- Grind solves the contradiction for us
           grind
+  -/
+
+example (b : UInt8) : b.toNat < 256 :=
+  b.toBitVec.isLt
+
+-- We'll need the theorems below to help `omega` in the `VarInt.parser_reconstruct`
+-- proof.
+private theorem UInt8.toNat_pos {b : UInt8} (h : ¬b = 0) : 0 < b.toNat := by
+  apply Nat.pos_of_ne_zero
+  intro h_zero
+  apply h
+  cases b
+  rename_i bv
+  have h_bv_eq_zero : bv = 0 := by
+    apply BitVec.eq_of_toNat_eq
+    exact h_zero
+  rw [h_bv_eq_zero]
+  rfl
+private theorem UInt8.toNat_lt_256 (b : UInt8) : b.toNat < 256 :=
+  b.toBitVec.isLt
+
+theorem VarInt.parser_reconstruct
+    (input : List UInt8) (v : VarInt) (rest : List UInt8) :
+    VarInt.parser.run input = some (v, rest) → input = v.serialize ++ rest := by
+
+  intro h_parse
+  have ⟨v', v_h⟩ := v
+  have h_cast : (↑(128 : VarInt) : Nat) = 128 := rfl
+
+  simp [VarInt.parser] at h_parse
+  unfold VarInt.parser.loop at h_parse
+  simp at h_parse
+  cases input with
+  | nil => contradiction
+  | cons b1 rest1 =>
+    simp [UInt8.parser] at h_parse
+    split at h_parse
+    · next h_128_leq_b1 =>
+      have h_128_leq_b1_nat : 128 ≤ b1.toNat := h_128_leq_b1
+      cases rest1 with
+      | nil => contradiction
+      | cons b2 rest2 =>
+        unfold parser.loop at h_parse
+        simp [UInt8.parser] at h_parse
+        split at h_parse
+        · contradiction
+        · next h_b2_neq_0 =>
+          have h_b2_neq_0_nat : 0 < b2.toNat := UInt8.toNat_pos h_b2_neq_0
+          split at h_parse
+          · next h_b2_leq_128 =>
+            have h_b2_leq_128_nat : 128 ≤ b2.toNat := h_b2_leq_128
+            cases rest2 with
+            | nil => contradiction
+            | cons b3 rest3 =>
+              unfold parser.loop at h_parse
+              simp [UInt8.parser] at h_parse
+              split at h_parse
+              · contradiction
+              · next h_b3_neq_0 =>
+                have h_b3_neq_0_nat : 0 < b3.toNat := UInt8.toNat_pos h_b3_neq_0
+                split at h_parse
+                · next h_128_leq_b3 =>
+                  have h_128_leq_b3_nat : 128 ≤ b3.toNat := h_128_leq_b3
+                  cases rest3 with
+                  | nil => contradiction
+                  | cons b4 rest4 =>
+                    unfold parser.loop at h_parse
+                    simp [UInt8.parser] at h_parse
+                    split at h_parse
+                    · contradiction
+                    · next h_b4_neq_0 =>
+                      have h_b4_neq_0_nat : 0 < b4.toNat := UInt8.toNat_pos h_b4_neq_0
+                      split at h_parse
+                      · next h_128_leq_b4 =>
+                        unfold parser.loop at h_parse
+                        contradiction
+                      · next h_128_gt_b4 =>
+                        have h_128_gt_b4_nat : ¬128 ≤ b4.toNat := h_128_gt_b4
+                        split at h_parse
+                        rotate_left
+                        · contradiction
+                        · next h_limit =>
+                          simp at h_parse
+                          obtain ⟨h_val, h_rest⟩ := h_parse
+                          rw [← h_rest]
+
+                          unfold VarInt.serialize
+                          have : ¬v' < 128 := by omega
+                          simp [dif_neg this]
+
+                          unfold VarInt.serialize; simp
+                          rw [h_cast]
+                          have : ¬v' / 128 < 128 := by omega
+                          simp [if_neg this]
+
+                          unfold VarInt.serialize
+                          simp
+                          rw [h_cast]
+                          have : ¬v' / 128 / 128 < 128 := by omega
+                          simp [if_neg this]
+
+                          unfold VarInt.serialize
+                          simp
+                          rw [h_cast]
+                          have : v' / 128 / 128 / 128 < 128 := by omega
+                          simp [if_pos this]
+
+                          refine ⟨?_, ?_, ?_, ?_⟩
+                          · apply UInt8.toNat.inj; simp
+                            have h_b1_limit := UInt8.toNat_lt_256 b1
+                            omega
+                          · apply UInt8.toNat.inj; simp
+                            have h_b2_limit := UInt8.toNat_lt_256 b2
+                            omega
+                          · apply UInt8.toNat.inj; simp
+                            have h_b2_limit := UInt8.toNat_lt_256 b3
+                            omega
+                          · apply UInt8.toNat.inj; simp
+                            have h_b2_limit := UInt8.toNat_lt_256 b4
+                            omega
+                · next h_b3_gt_128 =>
+                  have h_b3_gt_128 : ¬128 ≤ b3.toNat := h_b3_gt_128
+                  split at h_parse
+                  · next h_limit =>
+                    simp at h_parse
+                    obtain ⟨h_val, h_rest⟩ := h_parse
+                    rw [← h_rest]
+
+                    unfold VarInt.serialize; simp
+                    have : ¬v' < 128 := by omega
+                    simp [if_neg this]
+
+                    unfold VarInt.serialize; simp
+                    rw [h_cast]
+                    have : ¬v' / 128 < 128 := by omega
+                    simp [if_neg this]
+
+                    unfold VarInt.serialize; simp
+                    rw [h_cast]
+                    have : v' / 128 / 128 < 128 := by omega
+                    simp [if_pos this]
+
+                    refine ⟨?_, ?_, ?_⟩
+                    · apply UInt8.toNat.inj; simp
+                      have h_b1_limit := UInt8.toNat_lt_256 b1
+                      omega
+                    · apply UInt8.toNat.inj; simp
+                      have h_b2_limit := UInt8.toNat_lt_256 b2
+                      omega
+                    · apply UInt8.toNat.inj; simp
+                      have h_b3_limit := UInt8.toNat_lt_256 b3
+                      omega
+                  · contradiction
+          · next h_128_le_b2 =>
+            have h_128_le_b2_nat : ¬128 ≤ b2.toNat := h_128_le_b2
+            split at h_parse
+            · next h_limit =>
+              simp at h_parse
+              obtain ⟨h_val, h_rest⟩ := h_parse
+              rw [← h_rest]
+
+              unfold VarInt.serialize; simp
+              have : ¬v' < 128 := by omega
+              simp [if_neg this]
+
+              unfold VarInt.serialize; simp
+              rw [h_cast]
+              have : v' / 128 < 128 := by omega
+              simp [if_pos this]
+
+              refine ⟨?_, ?_⟩
+              · apply UInt8.toNat.inj; simp
+                have h_b1_limit := UInt8.toNat_lt_256 b1
+                omega
+              · apply UInt8.toNat.inj; simp
+                have h_b2_limit := UInt8.toNat_lt_256 b2
+                omega
+            · contradiction
+    · next h_128_gt_b1 =>
+      have h_128_gt_b1_nat : ¬128 ≤ b1.toNat := h_128_gt_b1
+      split at h_parse
+      · next h_limit =>
+        simp at h_parse
+        obtain ⟨h_val, h_rest⟩ := h_parse
+        rw [← h_rest]
+
+        unfold VarInt.serialize; simp
+        have : v' < 128 := by omega
+        simp [if_pos this]
+
+        apply UInt8.toNat.inj; simp
+        have h_b1_limit := UInt8.toNat_lt_256 b1
+        omega
+      · contradiction
 
 /--
   Executable checker: Returns true if 'n' survives the roundtrip.
